                    Ejercicios

Primer Ejercicio: [(¬P→Q)∧¬P]→Q

Segundo Ejercicio: ¬P∧[¬QV(P→Q)]

Soluciones:

Expresión lógica a resolver: [(¬P→Q)∧¬P]→Q

| P | Q | ¬P | ¬P→Q | (¬P→Q) ∧ ¬P | [(¬P→Q)∧¬P]→Q |
|---|---|----|------|-------------|---------------|
| V | V | F  |  V   |      F      |       V       |
| V | F | F  |  v   |      F      |       V       |
| F | V | V  |  v   |      v      |       V       |
| F | F | V  |  F   |      F      |       V       |


Expresión lógica a resolver: ¬P∧[¬QV(P→Q)]


| P | Q | ¬Q | P→Q | ¬QV(P→Q) |  ¬P |¬P∧[¬QV(P→Q)] |
|---|---|----|-----|----------|-----|--------------|
| V | V | F  |  V  |    V     |  F  |      F       |
| V | F | V  |  F  |    V     |  F  |      F       |
| F | V | F  |  v  |    v     |  V  |      V       |
| F | F | V  |  V  |    V     |  V  |      V       |


