                    Ejercicios

Primer Ejercicio: [(P↔Q)V(¬Q∧R)]↔(r→q)

Segundo Ejercicio: (P∧Q)→[(QVR)∧(P→¬Q)]


Soluciones:


Expresión lógica a resolver: [(P↔Q)V(¬Q∧R)]↔(r→q)

| P | Q | R | P→Q |¬Q | ¬Q∧R | (P↔Q)V(¬Q∧R) | r→q | [(P↔Q)V(¬Q∧R)]↔(r→q) |
|---|---|---|-----|---|------|--------------|-----|----------------------|
| V | V | V |  V  | F |   F  |      V       |  V  |         V            |
| V | V | F |  V  | F |   F  |      V       |  V  |         V            |
| V | F | V |  F  | V |   V  |      V       |  F  |         F            |
| V | F | F |  F  | V |   F  |      F       |  V  |         F            |
| F | V | V |  v  | F |   F  |      V       |  V  |         V            |
| F | V | F |  v  | F |   F  |      V       |  V  |         V            |
| F | F | V |  V  | V |   V  |      V       |  F  |         F            |
| F | F | F |  V  | V |   F  |      V       |  V  |         V            |

Expresión lógica a resolver: (P∧Q)→[(QVR)∧(P→¬Q)]


                         *       *                           
| P | Q | R | P∧Q |¬Q | P→¬Q | QVR | (QVR)∧(P→¬Q) | (P∧Q)→[(QVR)∧(P→¬Q)] |
|---|---|---|-----|---|------|-----|--------------|----------------------|
| V | V | V |  V  | F |   F  |  V  |       F      |         F            |
| V | V | F |  V  | F |   F  |  V  |       F      |         F            |
| V | F | V |  F  | V |   V  |  V  |       V      |         V            |
| V | F | F |  F  | V |   V  |  F  |       F      |         V            |
| F | V | V |  F  | F |   V  |  V  |       V      |         V            |
| F | V | F |  F  | F |   V  |  V  |       V      |         V            |
| F | F | V |  F  | V |   V  |  V  |       V      |         V            |
| F | F | F |  F  | V |   V  |  F  |       F      |         V            |




